Make connection table conditional on a model flag; extracts well

src/tls/experiments/ConnectionTable/Test.fst
@@ -5,7 +5,7 @@ open ConnectionTable
 
 open FStar.HyperStack.ST
 
-#set-options "--z3rlimit 100"
+#set-options "--z3rlimit 100"// --max_fuel 0 --max_ifuel 0"
 
 (*
    This tests the server side of a full handshake with mismatched parameters:
@@ -21,21 +21,36 @@ open FStar.HyperStack.ST
       b. Receive a ClientFinished on c2. Transition c2 to Complete 0 ch2 1
    8. Deallocate c2
 *)
+module T = FStar.Monotonic.DependentMap
+
 let test
   (cfg:configuration)
   (ch1:client_hello{~(has_cookie ch1) /\ ch_random ch1 == 0ul})
   (ch2:client_hello{has_cookie ch2 /\ ch_random ch2 == 0ul})
 : ST connection_table
   (requires fun _ ->
-    witnessed (region_contains_pred rgn) /\ ch_of_cookie ch2 == ch1 /\
+      witnessed (region_contains_pred rgn) /\ ch_of_cookie ch2 == ch1 /\
     ~(ch_compatible ch1 cfg))
-  (ensures  fun h0 t h1 -> inv t h1)
+  (ensures  fun h0 t h1 -> 
+    if model then 
+      let t:_connection_table = t in
+      inv t h1
+    else True)
 =
+  let id1:maybe_id = if model then 1ul else () in
+  let id2:maybe_id = if model then 2ul else () in
   let t = alloc () in
-  let c1 = create t 1ul cfg in
-  receive_client_hello1 t 1ul ch1;
-  free_connection t 1ul;
-  let c2 = create t 2ul cfg in
-  if receive_client_hello2 t 2ul ch2 then receive_client_finished t 2ul;
-  free_connection t 2ul;
+  let c1 = create t id1 cfg in
+  receive_client_hello1 t id1 c1 ch1;
+  free_connection t id1 c1;
+  let h1 = get () in
+  assert (
+    if model then
+      let t:_connection_table = t in
+      ~(T.defined t id2 h1)
+    else True);
+  let c2 = create t id2 cfg in
+  if receive_client_hello2 t id2 c2 ch2 then 
+    receive_client_finished t id2 c2;
+  free_connection t id2 c2;
   t
